src/Quine.v
@@ -1,0 +1,357 @@
+Require Import LC.Util.Fin.
+Require Import LC.Util.Vec.
+Require Import LC.Util.Star.
+Require Import LC.LC.
+Require Import LC.CNum.
+Require Import LC.Bool.
+Require Import LC.Tuple.
+Require Import LC.Combinators.
+Require Import LC.Interpreter.
+
+(* fun t1 t2 v a l => a (t1 v a l) (t2 v a l) *)
+
+Definition A {m} : Term m :=
+  Lam (Lam (Lam (Lam (Lam (
+    var 1 # (var 4 # var 2 # var 1 # var 0) # (var 3 # var 2 # var 1 # var 0)
+  ))))).
+
+Global Instance A_const : Const (@A).
+Proof.
+  constructor.
+  intros; reflexivity.
+Qed.
+
+Lemma app_reds {n} (T1 T2 U1 U2 : Term n) :
+  reds T1 T2 ->
+  reds U1 U2 ->
+  reds (T1 # U1) (T2 # U2).
+Proof.
+  intros.
+  eapply star_trans.
+  - apply app_reds_l; eauto.
+  - apply app_reds_r; auto.
+Qed.
+
+Lemma quote_with_vars {m n} (T : Term n) :
+  reds (quote T # var 2 # var 1 # var 0) ((@quote_aux m n T)).
+Proof.
+  unfold quote; simpl.
+  normal_order2.
+  induction T.
+  - simpl. subst_simpl.
+    repeat rewrite subst_const.
+    normal_order.
+  - simpl. subst_simpl.
+    apply app_reds.
+    + apply app_reds_r.
+      auto.
+    + auto.
+  - simpl. subst_simpl.
+    apply app_reds_r.
+    auto.
+Qed.
+
+Lemma A_reds {m n} (T1 T2 : Term n) :
+  reds ((A : Term m) # quote T1 # quote T2) (quote (T1 # T2)).
+Proof.
+  unfold A.
+  eapply R_star; [beta|].
+  subst_simpl.
+  repeat rewrite weaken_quote.
+  eapply R_star; [beta|].
+  subst_simpl.
+  repeat rewrite weaken_quote.
+  repeat rewrite subst_quote.
+  unfold quote at 3.
+  do 3 apply lam_reds.
+  simpl quote_aux.
+  eapply app_reds.
+  - apply app_reds_r.
+    apply quote_with_vars.
+  - apply quote_with_vars.
+Qed.
+
+Fixpoint quote_with_terms {m n} (t : Term n) (V A L : Term m) : Term m :=
+  match t with
+  | Var i => V # (cnum (nat_of_Fin i))
+  | t1 # t2 => A # quote_with_terms t1 V A L # quote_with_terms t2 V A L
+  | Lam t' => L # quote_with_terms t' V A L
+  end.
+
+Lemma quote_aux_quote_with_terms {m n} (t : Term n) :
+  (quote_aux t : Term (S (S (S m)))) =
+  quote_with_terms t (var 2) (var 1) (var 0).
+Proof.
+  induction t.
+  - simpl. auto.
+  - simpl. rewrite IHt1, IHt2. auto.
+  - simpl. rewrite IHt. auto.
+Qed.
+
+Lemma quote_with_terms_subst {m n} (t : Term n) (V A L : Term (S m))
+  (i : Fin (S m)) (U : Term m) :
+  subst (quote_with_terms t V A L) i U =
+  quote_with_terms t (subst V i U) (subst A i U) (subst L i U).
+Proof.
+  induction t.
+  - simpl; subst_simpl.
+    now rewrite subst_const.
+  - simpl; subst_simpl.
+    congruence.
+  - simpl; subst_simpl.
+    congruence.
+Qed.
+
+Definition NQhat {m} : Term m :=
+  Lam (Lam (Lam (Lam
+    (var 0 # (var 2 # (var 3 # cnum 1)) # (var 3 # cnum 0))))).
+
+Global Instance NQhat_const : Const (@NQhat).
+Proof.
+  constructor; intros; reflexivity.
+Qed.
+
+Definition NQ {m} : Term m :=
+  Lam (Lam (Lam (Lam
+    (var 1 # (var 1 # (NQhat # var 3  # var 2 # var 1 # var 0)))))).
+
+Global Instance NQ_const : Const (@NQ).
+Proof.
+  constructor; intros; reflexivity.
+Qed.
+
+Lemma NQ_correct {m} (A B C : Term m) n :
+  reds (NQ # A # B # C # (cnum n)) (quote_with_terms (cnum n : Term m) A B C).
+Proof.
+  unfold NQ.
+  normal_order2.
+  do 2 apply app_reds_r.
+  unfold NQhat.
+  normal_order2.
+  eapply star_trans; [apply cnum_reds|].
+  induction n.
+  - apply star_refl.
+  - simpl; apply app_reds_r.
+    auto.
+Qed.
+
+Definition VQ {m} : Term m :=
+  Lam (Lam (Lam (Lam (var 2 # (var 3 # cnum 2) # (NQ # var 3 # var 2 # var 1 # var 0))))).
+
+Global Instance VQ_const : Const (@VQ).
+Proof.
+  constructor; intros; reflexivity.
+Qed.
+
+Definition AQ {m} : Term m :=
+  Lam (Lam (Lam (Lam (var 2 # (var 2 # (var 3 # cnum 1) # var 0))))).
+
+Global Instance AQ_const : Const (@AQ).
+Proof.
+  constructor; intros; reflexivity.
+Qed.
+
+Definition LQ {m} : Term m :=
+  Lam (Lam (Lam (var 1 # (var 2 # cnum 0)))).
+
+Global Instance LQ_const : Const (@LQ).
+Proof.
+  constructor; intros; reflexivity.
+Qed.
+
+Definition Qhat {m} : Term m :=
+  Lam (Lam (Lam (Lam
+    (var 3 #
+      (VQ # var 2 # var 1 # var 0) #
+      (AQ # var 2 # var 1 # var 0) #
+      (LQ # var 2 # var 1 # var 0))))).
+
+Global Instance Qhat_const : Const (@Qhat).
+Proof.
+  constructor; intros; reflexivity.
+Qed.
+
+Definition Q {m} : Term m :=
+  Lam (Lam (Lam (Lam
+    (var 0 # (var 0 # (var 0 # (Qhat # var 3 # var 2 # var 1 # var 0))))))).
+
+Global Instance QQ_const : Const (@Q).
+Proof.
+  constructor; intros; reflexivity.
+Qed.
+
+Lemma quote_aux_app {m n} (T1 T2 : Term n) :
+  (quote_aux (T1 # T2) : Term (S (S (S m)))) =
+  var 1 # quote_aux T1 # quote_aux T2.
+Proof.
+  auto.
+Qed.
+
+Lemma quote_aux_lam {m n} (T : Term (S n)) :
+  (quote_aux (Lam T) : Term (S (S (S m)))) =
+  var 0 # quote_aux T.
+Proof.
+  auto.
+Qed.
+
+Lemma quote_var {m} {n} (i : Fin n) :
+  (quote (Var i) : Term m) = Lam (Lam (Lam (var 2 # (cnum (nat_of_Fin i))))).
+Proof.
+  auto.
+Qed.
+
+Lemma weaken_Var {n} (i : Fin n) (j : Fin (S n)) :
+  weaken (Var i) j = Var (shift j i).
+Proof.
+  auto.
+Qed.
+
+Lemma weaken_App {n} (T1 T2 : Term n) (j : Fin (S n)) :
+  weaken (T1 # T2) j = weaken T1 j # weaken T2 j.
+Proof.
+  auto.
+Qed.
+
+Lemma weaken_Lam {n} (T : Term (S n)) (j : Fin (S n)) :
+  weaken (Lam T) j = Lam (weaken T (inr j)).
+Proof.
+  auto.
+Qed.
+
+(*
+Lemma Qhat_reds {m n} (T : Term n) :
+  reds  T T.
+*)
+
+Lemma Q_reds {m n} (T : Term n) :
+  reds ((Q : Term m) # quote T) (quote (quote T : Term m)).
+Proof.
+  unfold Q.
+  eapply R_star; [beta|].
+  subst_simpl.
+  do 3 apply lam_reds.
+  simpl quote_aux at 1.
+  do 3 apply app_reds_r.
+  repeat rewrite weaken_quote.
+  rewrite subst_const.
+  unfold Qhat.
+  eapply R_star; [beta|].
+  subst_simpl.
+  repeat rewrite weaken_quote.
+  repeat rewrite subst_const.
+  eapply R_star; [beta|].
+  subst_simpl.
+  repeat rewrite subst_quote.
+  repeat rewrite subst_const.
+  simpl weaken.
+  eapply R_star; [beta|].
+  subst_simpl.
+  repeat rewrite subst_quote.
+  repeat rewrite subst_const.
+  simpl weaken.
+  eapply R_star; [beta|].
+  subst_simpl.
+  repeat rewrite subst_quote.
+  repeat rewrite subst_const.
+  unfold quote.
+  eapply R_star; [beta|].
+  subst_simpl.
+  repeat rewrite weaken_app.
+  repeat rewrite weaken_const.
+  simpl weaken.
+  eapply R_star; [beta|].
+  subst_simpl.
+  repeat rewrite weaken_app.
+  repeat rewrite weaken_const.
+  simpl weaken.
+  eapply R_star; [beta|].
+  rewrite quote_aux_quote_with_terms.
+  unfold var.
+  rewrite @quote_with_terms_subst.
+  subst_simpl.
+  rewrite @quote_with_terms_subst.
+  subst_simpl.
+  rewrite @quote_with_terms_subst.
+  subst_simpl.
+  repeat rewrite subst_const.
+  induction T.
+  - simpl.
+    unfold VQ.
+    normal_order2.
+    apply app_reds_r.
+    eapply star_trans; [apply NQ_correct|].
+    unfold cnum; simpl.
+    rewrite quote_aux_quote_with_terms.
+    normal_order.
+  - simpl.
+    unfold AQ.
+    normal_order2.
+    apply app_reds; auto.
+    do 2 apply app_reds_r.
+    auto.
+  - simpl.
+    unfold LQ.
+    normal_order2.
+    apply app_reds; auto.
+    apply star_refl.
+Qed.
+
+Definition pre_KFP {m} (P : Term m) : Term m.
+Proof.
+  apply Lam.
+  apply App.
+  - exact (weaken P (inl tt)).
+  - apply App.
+    + apply App.
+      * exact A.
+      * exact (var 0).
+    + apply App.
+      * exact Q.
+      * exact (var 0).
+Defined.
+
+Definition KFP {m} (P : Term m) : Term m :=
+  (pre_KFP P) # quote (pre_KFP P).
+
+Theorem Kleene_Recursion_Thm {m} (P : Term m) :
+  reds (KFP P) (P # quote (KFP P)).
+Proof.
+  pose (QP := pre_KFP P).
+  unfold KFP at 1.
+  unfold pre_KFP at 1.
+  fold QP.
+  apply star_trans with (y := P # (A # quote QP # (Q # quote QP))).
+  - normal_order2.
+  - apply app_reds_r.
+    eapply star_trans with (y := A # quote QP # (quote (quote QP))).
+    + apply app_reds_r.
+      apply Q_reds.
+    + apply A_reds.
+Qed.
+
+Definition I_comb {n} : Term n :=
+  Lam (var 0).
+
+Lemma I_reds {n} (T : Term n) :
+  reds (I_comb # T) T.
+Proof.
+  unfold I_comb.
+  normal_order2.
+Qed.
+
+Definition Quine : Term 0 :=
+  KFP I_comb.
+
+Theorem Quine_correct :
+  reds Quine (quote Quine).
+Proof.
+  eapply star_trans.
+  - apply Kleene_Recursion_Thm.
+  - apply I_reds.
+Qed.
+
+Set Printing Depth 1000000.
+Require Import String.
+
+Eval vm_compute in Quine.
+Eval vm_compute in print_term Quine.
